Define switcher invariant, starting up the proof (ish)

theories/examples/switcher/switcher_spec.v
@@ -35,9 +35,25 @@ Section Switcher.
        A possibility is to use a resource that encodes it.
      - Where is the code? Where is MTDC and trusted stack?
        We need to have a switcher state invariant.
+     - reverse the stack, for simplicity ?
    *)
+
+  Definition switcher_inv
+    (b_switcher e_switcher a_switcher_cc : Addr)
+    (ot_switcher : OType) : iProp Σ :=
+    ∃ (b_tstk e_tstk a_tstk : Addr) (tstk : list Word),
+     mtdc ↦ₛᵣ WCap RWL Local b_tstk e_tstk a_tstk
+     ∗ ⌜ SubBounds
+         b_switcher e_switcher
+         a_switcher_cc (a_switcher_cc ^+ length switcher_instrs)%a ⌝
+     ∗ codefrag a_switcher_cc switcher_instrs
+     ∗ b_switcher ↦ₐ WSealRange (true,true) Global ot_switcher (ot_switcher^+1)%ot ot_switcher
+     ∗ [[ a_tstk, e_tstk ]] ↦ₐ [[ tstk ]]
+  .
+
+
   Lemma switcher_cc_specification
-    (E : coPset)
+    (E : coPset) (N : namespace)
     (W0 W1 : WORLD)
     (C : CmptName)
     (g_switcher : Locality)
@@ -52,8 +68,11 @@ Section Switcher.
 
     is_arg_rmap arg_rmap ->
     dom rmap = all_registers_s ∖ ((dom arg_rmap) ∪ {[ PC ; cgp ; cra ; csp ; cs0 ]} ) ->
-    (
-      PC ↦ᵣ WCap XSRW_ g_switcher b_switcher e_switcher a_switcher_cc
+    ↑N ⊆ E →
+
+    ( na_inv logrel_nais N (switcher_inv b_switcher e_switcher a_switcher_cc ot_switcher)
+      ∗ na_own logrel_nais E
+      ∗ PC ↦ᵣ WCap XSRW_ g_switcher b_switcher e_switcher a_switcher_cc
       ∗ cgp ↦ᵣ wcgp_caller
       ∗ cra ↦ᵣ wcra_caller
       ∗ csp ↦ᵣ WCap RWL Local b_stk e_stk a_stk
@@ -61,6 +80,7 @@ Section Switcher.
       ∗ ( [∗ map] rarg↦warg ∈ arg_rmap, rarg ↦ᵣ warg ∗ interp W1 C warg )
       ∗ ( [∗ map] r↦w ∈ rmap, r ↦ᵣ w )
 
+      (* TODO the stack is reversed! so actually, we have [[ b_stk_, a_stk ]] *)
       ∗ [[ a_stk , e_stk ]] ↦ₐ [[ stk_mem ]]
 
       ∗ region W0 C ∗ sts_full_world W0 C
@@ -71,6 +91,7 @@ Section Switcher.
       ∗ ▷ ( ∃ (W2 : WORLD) (rmap' : Reg),
               ⌜ related_sts_pub_world W1 W2 C ⌝
               ∗ ⌜ dom rmap' = all_registers_s ∖ {[ PC ; cgp ; cra ; csp ; ca0 ; ca1 ]} ⌝
+              ∗ na_own logrel_nais E
               ∗ region W2 C ∗ sts_full_world W2 C
               ∗ PC ↦ᵣ updatePcPerm wcra_caller
               ∗ cgp ↦ᵣ wcgp_caller ∗ (∃ wret, cra ↦ᵣ wret)
@@ -82,8 +103,67 @@ Section Switcher.
             -∗ WP Seq (Instr Executable) {{ φ }}
           )
     )
-    ⊢ WP Seq (Instr Executable) {{ λ v, φ v ∨ ⌜v = FailedV⌝ }}%I.
+    ⊢ (WP Seq (Instr Executable) {{ λ v, φ v ∨ ⌜v = FailedV⌝ }})%I.
   Proof.
+    intros Harg_map Hrmap HNE Hbounds.
+    iIntros "(#Hinv_switcher & Hna
+              & HPC & Hcgp & Hcra & Hcsp & Hcs0 & Hargmap & Hrmap
+              & Hstk & Hregion & Hworld & Hnext_world & Hcont)".
+
+    (* ------------------------------------------------ *)
+    (* -------- Prepare resources for the proof ------- *)
+    (* ------------------------------------------------ *)
+
+    (* --- Extract the code from the invariant --- *)
+    iMod (na_inv_acc with "Hinv_switcher Hna")
+      as "(Hswitcher_inv & Hna & Hclose_switcher_inv)" ; auto.
+    rewrite /switcher_inv.
+    iDestruct "Hswitcher_inv"
+      as (b_tstk e_tstk a_tstk tstk) ">(Hmtdc & Hcode & Hb_switcher & Htstk)".
+    codefrag_facts "Hcode".
+    rename H into Hcont_switcher_region; clear H0.
+
+    (* --- Extract scratch registers cs1 ct2 --- *)
+    (* TODO *)
+    assert (exists wcs1, rmap !! cs1 = Some wcs1) as [wcs1 Hwcs1].
+    { admit. }
+    assert (exists wct2, rmap !! ct2 = Some wct2) as [wct2 Hwct2].
+    { admit. }
+    iDestruct (big_sepM_delete _ _ cs1 with "Hrmap") as "[Hcs1 Hrmap]"; first eassumption.
+    iDestruct (big_sepM_delete _ _ ct2 with "Hrmap") as "[Hct2 Hrmap]"; first by simplify_map_eq.
+    (* ------------------------------------------------ *)
+    (* ----- Start the proof of the switcher here ----- *)
+    (* ------------------------------------------------ *)
+
+    (* ---- store csp cs0 ---- *)
+    destruct (stk_mem) as [|stk_a stk_mem0].
+    { (* memory overflow ? *) admit. }
+    (* memory overflow ? *)
+    iDestruct (region_pointsto_cons with "Hstk") as "[Ha_stk Hstk]".
+    { transitivity (Some (a_stk ^+ 1)%a); auto. admit. }
+    { admit. }
+    destruct ( withinBounds b_stk e_stk a_stk ) eqn:Hastk_inbounds; cycle 1.
+    { (* if a_stk is not in bounds, fail *)
+      admit.
+    }
+    iInstr "Hcode".
+    { admit. (* TODO RWL can store everything, make a lemma and add it as a hint *) }
+
+
+    (* ---- lea csp (-1) ---- *)
+    iInstr "Hcode".
+    { transitivity (Some (a_stk ^+ (-1)%Z)%a); auto. admit. }
+
+    (* ---- store csp cs1 ---- *)
+    destruct (stk_mem0) as [|stk_a1 stk_mem1].
+    { (* memory overflow ? *) admit. }
+    (* memory overflow ? *)
+    iDestruct (region_pointsto_cons with "Hstk") as "[Ha1_stk Hstk]".
+    { transitivity (Some (a_stk ^+ 2)%a); auto. admit. }
+    { admit. }
+    iInstr "Hcode".
+
+
   Admitted.
 
 
